theories/c_toy_lang/melocoton/mlang_instantiation.v
@@ -1,0 +1,13 @@
+From stdpp Require Export binders strings.
+From stdpp Require Import gmap.
+From iris.algebra Require Export ofe.
+From iris.heap_lang Require Export locations.
+From iris.prelude Require Import options.
+From melocoton.mlanguage Require Export mlanguage.
+From melocoton.c_toy_lang Require Export lang metatheory.
+From melocoton.c_toy_lang.melocoton Require Import lang_instantiation.
+From melocoton.interop Require Import lang_to_mlang.
+
+Canonical Structure C_mlang := (lang_to_mlang C_lang).
+
+
