theories/examples/even_odd.v
@@ -87,6 +87,7 @@ End specs.
 
 From melocoton.interop Require Import linking linking_wp lang_to_mlang_wp.
 From melocoton.mlanguage Require Import weakestpre.
+From melocoton.c_toy_lang.melocoton Require Import mlang_instantiation.
 
 Section linking.
 Context `{!heapGS_C Σ, !invGS_gen hlc Σ}.
