theories/interop/lang_to_mlang.v
@@ -33,9 +33,6 @@ Section ToMlang.
   Definition is_call (e : Λ.(expr)) (s : string) (vs : list val) (C : cont) : Prop := 
     e = fill C (of_class Λ (ExprCall s vs)).
 
-  Definition XM_for (P:Prop) : Prop := P ∨ ¬ P.
-  Axiom (XM_for_reducible : ∀ p e σ, XM_for (reducible (Λ:=Λ) p e σ)).
-
   Lemma language_mlanguage_mixin :
     MlanguageMixin (val:=val) (of_val Λ) to_val is_call (fill) (Λ.(comp_ectx)) (Λ.(apply_func)) prim_step.
   Proof using.
@@ -62,14 +59,15 @@ Section ToMlang.
     - intros e C1 C2 s vv Heq. rewrite /is_call -fill_comp. by f_equal.
     - intros e C. apply fill_val.
     - intros e C1 C2. apply fill_comp.
+    - by intros e s1 s2 f1 f2 C1 C2 -> (->&->&->)%call_call_in_ctx.
     - intros p C e σ X Hnv. inversion 1; simplify_eq.
       + apply fill_step_inv in H3 as (e2'&->&HH); last done.
         by eapply LiftStep.
       + destruct H4 as [Hnv2 Hstuck].
         eapply LiftUbStep; split; first done.
         intros e2 σ2 Hc. eapply Hstuck, fill_prim_step, Hc.
-    - intros p e σ H.
-      destruct (XM_for_reducible p e σ) as [(e2&σ2&Hl)|Hr].
+    - intros p e σ XM H.
+      destruct (XM ((reducible (Λ:=Λ) p e σ))) as [(e2&σ2&Hl)|Hr].
       + eapply LiftStep; last done. exact Hl.
       + eapply LiftUbStep. split; first done. intros ? ? ?. eapply Hr. by do 2 eexists.
   Qed.
@@ -79,11 +77,10 @@ Section ToMlang.
 
   Inductive lang_to_mlang_split_state : Λ.(state) → Λ.(state) → unit → Prop :=
     split_state_refl σ : lang_to_mlang_split_state σ σ ().
-(*
+
   Global Program Instance lang_to_mlang_linkable : linkable lang_to_mlang Λ.(state) := {
     linking.private_state := unit;
     linking.split_state := lang_to_mlang_split_state;
   }.
-  Next Obligation. intros *. inversion 1; inversion 1; by simplify_eq. Qed.
- *)
+
 End ToMlang.
